Semantics.v
@@ -1,5 +1,11 @@
 Require Import List.
 
+Require Import Vpl.Impure.
+Require Import Mymap.
+Require Import ImpureOperations.
+
+Require Import Misc.
+
 Parameter mem : Type.
 
 (** * Iterating semantics on a list *)
@@ -21,3 +27,83 @@ Proof.
   - simpl; auto.
   - intros; apply Himp; simpl; auto.
 Qed.
+
+Lemma iter_semantics_mapl :
+  forall (A B : Type) P (f : A -> B) (l : list A) mem1 mem2,
+    iter_semantics P (map f l) mem1 mem2 <-> iter_semantics (fun x => P (f x)) l mem1 mem2.
+Proof.
+  intros A B P f. induction l.
+  - intros; split; simpl; intros H; inversion_clear H; constructor.
+  - intros; split; simpl; intros H; inversion_clear H; econstructor; eauto; rewrite IHl in *; auto.
+Qed.
+
+Lemma iter_semantics_combine :
+  forall (A B : Type) P (xs : list A) (ys : list B) mem1 mem2,
+    length xs = length ys -> iter_semantics P xs mem1 mem2 <-> iter_semantics (fun p => P (fst p)) (combine xs ys) mem1 mem2.
+Proof.
+  intros A B P xs ys mem1 mem2 H.
+  replace xs with (map fst (combine xs ys)) at 1 by (apply map_combine; auto).
+  rewrite iter_semantics_mapl; reflexivity.
+Qed.
+
+Module IterImpureSemantics (Import Imp: FullImpureMonad).
+
+  Module ImpOps := ImpureOps Imp.
+  Import ImpOps.
+
+  Lemma iter_semantics_sequence :
+    forall (A : Type) P (xs : list (imp A)) (ys : list A) mem1 mem2,
+      mayReturn (sequence xs) ys ->
+      iter_semantics (fun x mem3 mem4 => WHEN y <- x THEN P y mem3 mem4) xs mem1 mem2 -> iter_semantics P ys mem1 mem2.
+  Proof.
+    intros A P. induction xs.
+    - intros ys mem1 mem2 Hys Hsem; simpl in *. apply mayReturn_pure in Hys; rewrite <- Hys.
+      inversion_clear Hsem; constructor.
+    - intros ys mem1 mem2 Hys Hsem; simpl in *.
+      bind_imp_destruct Hys y Hy.
+      bind_imp_destruct Hys ys1 Hys1.
+      apply mayReturn_pure in Hys; rewrite <- Hys in *.
+      inversion_clear Hsem. 
+      econstructor; [apply H; auto|].
+      apply IHxs; auto.
+  Qed.
+
+  (* yet another unfortunately needed lemma because of mymap... *)
+  Lemma iter_semantics_mymapl :
+    forall (A B : Type) P (f : A -> B) (l : list A) mem1 mem2,
+      iter_semantics P (mymap f l) mem1 mem2 <-> iter_semantics (fun x => P (f x)) l mem1 mem2.
+  Proof.
+    intros A B P f. induction l.
+    - intros; split; simpl; intros H; inversion_clear H; constructor.
+    - intros; split; simpl; intros H; inversion_clear H; econstructor; eauto; rewrite IHl in *; auto.
+  Qed.
+
+  Lemma iter_semantics_mapM :
+    forall (A B : Type) f P (xs : list A) (ys : list B) mem1 mem2,
+      mayReturn (mapM f xs) ys ->
+      iter_semantics (fun x mem3 mem4 => WHEN y <- f x THEN P y mem3 mem4) xs mem1 mem2 -> iter_semantics P ys mem1 mem2.
+  Proof.
+    intros A B f P xs ys mem1 mem2 Hmap Hsem.
+    eapply iter_semantics_sequence; [exact Hmap|].
+    rewrite iter_semantics_mymapl. auto.
+  Qed.
+
+  Lemma iter_semantics_mapM_rev :
+    forall (A B : Type) P f (xs : list A) (ys : list B) mem1 mem2,
+      mayReturn (mapM f xs) ys ->
+      iter_semantics P ys mem1 mem2 ->
+      iter_semantics (fun '(x, y) mem3 mem4 => mayReturn (f x) y /\ P y mem3 mem4) (combine xs ys) mem1 mem2.
+  Proof.
+    intros A B P f. induction xs.
+    - intros ys mem1 mem2 Hys Hsem; simpl in *. apply mayReturn_pure in Hys; rewrite <- Hys in Hsem.
+      inversion_clear Hsem; constructor.
+    - intros ys mem1 mem2 Hys Hsem; simpl in *.
+      bind_imp_destruct Hys y Hy.
+      bind_imp_destruct Hys ys1 Hys1.
+      apply mayReturn_pure in Hys; rewrite <- Hys in *.
+      inversion_clear Hsem.
+      econstructor; [eauto|].
+      apply IHxs; auto.
+  Qed.
+
+End IterImpureSemantics.
